execution_invariants2.thy
@@ -1,5 +1,5 @@
 theory execution_invariants2
-  imports repliss_sem execution_invariants consistency commutativity
+  imports repliss_sem execution_invariants consistency commutativity "fuzzyrule.fuzzyrule"
 begin
 
 
@@ -12,7 +12,6 @@ lemma wf_generated_ids_invocation_exists:
   assumes wf: "state_wellFormed S"
 and "invocationOp S i = None"
 shows "generatedIds S uid \<noteq> Some i"
-  find_theorems name: induct state_wellFormed
   using assms proof (induct rule: wellFormed_induct)
   case initial
   then show ?case by (simp add: initialState_def)
@@ -21,7 +20,108 @@ next
   then show ?case by (auto simp add: initialState_def step.simps wf_localState_to_invocationOp split: if_splits)
 qed
 
+text "Every query can be explained with the corresponding query specification.
 
+"
+
+
+lemma wf_queryspec:
+  assumes wf: "state_wellFormed S"
+    and "calls S c \<triangleq> Call op r"
+    and "prevCalls = {c'. (c',c)\<in>happensBefore S}"
+    and "ctxt = getContextH (calls S |` prevCalls) (happensBefore S |r prevCalls) (Some prevCalls)"
+  shows "querySpec (prog S) op ctxt r"
+  using assms proof (induct rule: wellFormed_induct)
+  case initial
+  then show ?case 
+    by (simp add: initialState_def)
+next
+  case (step S1 a S2)
+  from ` S1 ~~ a \<leadsto> S2`
+  show ?case
+  proof (cases rule: step.cases)
+    case (local i ls f ls')
+    then show ?thesis 
+      using step by auto
+  next
+    case (newId i ls f ls' uid uidv ls'')
+    then show ?thesis using step by auto
+  next
+    case (beginAtomic i ls f ls' t vis snapshot)
+    then show ?thesis using step by auto
+  next
+    case (endAtomic i ls f ls' t)
+    then show ?thesis using step by auto
+  next
+    case (dbop i ls f Op ls' t c' res vis)
+    have [simp]: "prog S2 = prog S1"
+      using prog_inv step.hyps(3) by blast
+
+
+    show ?thesis 
+    proof (cases "c = c'")
+      case True
+
+      have [simp]: "(c', c) \<notin> happensBefore S1" for c
+        using local.dbop(7) step.hyps(1) wellFormed_happensBefore_calls_l by blast
+      have [simp]: "(c, c') \<notin> happensBefore S1" for c
+        using local.dbop(7) step.hyps(1) wellFormed_happensBefore_calls_r by blast
+      have [simp]: "c' \<notin> vis"
+        using local.dbop(7) local.dbop(9) step.hyps(1) wellFormed_visibleCallsSubsetCalls2 by blast
+
+
+      have "ctxt = getContext S1 i"
+        by (auto simp add: step dbop True getContextH_def operationContext_ext restrict_map_def
+            restrict_relation_def
+            intro!: ext
+            split: option.splits)
+
+
+      with `querySpec (prog S1) Op (getContext S1 i) res`
+      show ?thesis 
+        using `calls S2 c \<triangleq> Call op r`
+        by (simp add: dbop True)
+
+    next
+      case False
+      show ?thesis 
+      proof (simp add: step, fuzzy_rule step.hyps; (simp add: step dbop False; fail)?)
+        show "calls S1 c \<triangleq> Call op r"
+          using `calls S2 c \<triangleq> Call op r`
+          by (simp add: dbop False)
+
+        have [simp]: "c' \<notin> prevCalls"
+          using False `calls S1 c' = None` wellFormed_happensBefore_calls_l[OF `state_wellFormed S1`]
+          by (auto simp add: step dbop, blast)
+
+
+
+        have h1: "(calls S2 |` prevCalls) = (calls S1 |` prevCalls)"
+          by (auto simp add: restrict_map_def dbop False ) 
+
+        have h2: "happensBefore S2 |r prevCalls = happensBefore S1 |r prevCalls"
+          by (auto simp add: restrict_relation_def dbop False) 
+
+        show "ctxt = getContextH (calls S1 |` prevCalls) (happensBefore S1 |r prevCalls) (Some prevCalls)"
+          by (simp add: h1 h2 step.prems(3))
+      qed
+    qed
+
+  next
+    case (invocation i proc initialState impl)
+    then show ?thesis using step by auto
+  next
+    case (return i ls f res)
+    then show ?thesis using step by auto
+  next
+    case (fail i ls)
+    then show ?thesis using step by auto
+  next
+    case (invCheck res i)
+    then show ?thesis using step by auto
+  qed
+    
+qed
 
 
 end
